progress on destruct tactic

template-coq/theories/Tactics.v
@@ -9,8 +9,10 @@ Local Set Universe Polymorphism.
 Unset Guard Checking.
 
 Inductive tactic_result A : Type :=
-  | TacticSuccess : A -> tactic_result A 
-  | TacticError : tactic_result A.
+  (** A successful tactic. *)
+  | TacticSuccess : A -> tactic_result A
+  (** A failing tactic, with an error message. *) 
+  | TacticError : doc unit -> tactic_result A.
 Arguments TacticSuccess {A}%_type_scope a.
 Arguments TacticError {A}%_type_scope.
 
@@ -35,15 +37,15 @@ Instance monad_TacticM : Monad TacticM :=
     fun env nctx evm goals =>
       match mx env nctx evm goals with 
       | TacticSuccess (x, evm, goals) => mf x env nctx evm goals
-      | TacticError => TacticError
+      | TacticError err => TacticError err
       end
 }.
 
 (** * Basic TacticM bookkeeping. *)
 
 (** [fail_tac] is a tactic which always fails. *)
-Definition fail_tac {A} : TacticM A :=
-  fun _ _ _ _ => TacticError.
+Definition fail_tac {A} (err : doc unit) : TacticM A :=
+  fun _ _ _ _ => TacticError err.
 
 (** Fetch the global environment. *)
 Definition get_global_env : TacticM global_env :=
@@ -73,11 +75,28 @@ Definition get_goals : TacticM (list evar) :=
 Definition set_goals (goals : list evar) : TacticM unit :=
   fun env nctx evm _ => TacticSuccess (tt, evm, goals).
 
+(** [abstract x t] replaces all occurences of [tVar x] by [tRel 0] (modulo lifting) in [t]. *)
+Definition abstract (x : ident) (t : term) : term :=
+  let fix aux depth t :=
+    match t with 
+    | tVar x' => if x == x' then tRel depth else tVar x'
+    | _ => map_term_with_binders 0 (fun _ => S) aux t
+    end
+  in 
+  aux 0 t.
+
+(** Get the evar id in a term of the form [tEvar _ _]. *)
+Definition get_evar_id (t : term) : evar :=
+  match t with 
+  | tEvar ev _ => ev 
+  | _ => 0
+  end.
+
 (** Fetch the main goal (and fail if there are no goals). *)
 Definition get_main_goal : TacticM evar :=
   fun env nctx evm goals => 
     match goals with
-    | [] => TacticError 
+    | [] => TacticError $ str "get_main_goal : no goals"
     | g :: goals => TacticSuccess (g, evm, g :: goals)
     end.
 
@@ -85,20 +104,17 @@ Definition get_main_goal : TacticM evar :=
 Definition with_evar_context {A} (ev : evar) (t : TacticM A) : TacticM A :=
   mlet evm <- get_evar_map ;;
   match EvarMap.lookup evm ev with 
-  | None => fail_tac 
+  | None => fail_tac $ str "with_evar_context : undeclared evar"
   | Some entry => with_named_context entry.(ev_nctx) t
   end.
 
-(** [main_concl] returns the conclusion of the main goal,
-    and fails if there are no goals. *)
-Definition main_concl : TacticM term :=
-  mlet evm <- get_evar_map ;;
-  mlet goal <- get_main_goal ;;
-  match EvarMap.lookup evm goal with 
-  | None => fail_tac 
-  | Some entry => ret $ tEvar goal $ map (tVar <<< fst) entry.(ev_nctx)
+(** [with_main_context t] executes tactic [t] in the context of the main goal. *)
+Definition with_main_context {A} (t : TacticM A) : TacticM A :=
+  mlet goals <- get_goals ;;
+  match goals with 
+  | goal :: _ => with_evar_context goal t
+  | [] => fail_tac $ str "with_main_context : no goals"
   end.
-
 
 (** Tactics which don't require a goal. *)
 
@@ -139,8 +155,8 @@ Definition fresh_evar (basename : ident) (ty_opt : option term) : TacticM term :
   ;;
   (* Create ?x. *)
   fresh_evar_aux ty.
-  
-(** [typeof_tac t] computes the type of [t], assuming it is well-typed.
+
+(** [typeof_tac t] computes the type of [t] in the current context, assuming it is well-typed.
     If [t] is not well-typed, it might (but won't necessarily) fail. *)
 Definition typeof_tac (t : term) : TacticM term :=
   mlet env <- get_global_env ;;
@@ -148,8 +164,16 @@ Definition typeof_tac (t : term) : TacticM term :=
   mlet evm <- get_evar_map ;;
   match retype evm env nctx [] t with 
   | Checked ty => ret ty 
-  | TypeError _ => fail_tac
+  | TypeError _ => fail_tac $ str "typeof_tac : type error"
   end.
+
+(** [whnf_tac flags t] computes the weak-head normal form of [t] 
+    with reduction flags [flags]. *)
+Definition whnf_tac (flags : RedFlags.t) (t : term) : TacticM term :=
+  mlet env <- get_global_env ;;
+  mlet nctx <- get_named_context ;;
+  mlet evm <- get_evar_map ;;
+  ret $ weak_head_reduce flags evm env nctx [] t.
 
 (** [unify_tac flags pb t1 t2] unifies [t1] and [t2] using unification flags [flags]
     and conversion relation [pb], in the current named context.
@@ -168,10 +192,21 @@ Definition unify_tac (flags : UnifFlags.t) (pb : conv_pb) (t1 t2 : term) : Tacti
     It fails if [ev] is already assigned. *)
 Definition assign_tac (ev : evar) (t : term) : TacticM unit :=
   mlet evm <- get_evar_map ;; 
-  if EvarMap.is_defined evm ev then fail_tac
+  if EvarMap.is_defined evm ev 
+  then fail_tac $ str "assign_tac : evar is already assigned"
   else set_evar_map $ EvarMap.define evm ev t.
 
 (** * Tactics which work on a goal. *)
+
+(** [main_concl] returns the conclusion of the main goal,
+    and fails if there are no goals. *)
+Definition main_concl : TacticM term :=
+  mlet evm <- get_evar_map ;;
+  mlet goal <- get_main_goal ;;
+  match EvarMap.lookup evm goal with 
+  | None => fail_tac $ str "main_concl : undefined evar"
+  | Some entry => typeof_tac =<< tEvar goal $ map (tVar <<< fst) entry.(ev_nctx)
+  end.
 
 (** [simple_tactic t] is a tactic which applies [t] on the main goal (the first in the list).
     [t] returns a list of new goals, which replace the main goal.
@@ -179,28 +214,11 @@ Definition assign_tac (ev : evar) (t : term) : TacticM unit :=
 Definition simple_tactic {A} (t : evar -> TacticM (A * list evar)) : TacticM A :=
   mlet goals <- get_goals ;;
   match goals with 
-  | [] => fail_tac 
+  | [] => fail_tac $ str "simple_tactic : no goals"
   | g :: goals => 
     mlet (a, new_goals) <- with_evar_context g (t g) ;;
     set_goals (new_goals ++ goals) ;;
     ret a
-  end.
-
-(** [abstract x t] replaces all occurences of [tVar x] by [tRel 0] (modulo lifting) in [t]. *)
-Definition abstract (x : ident) (t : term) : term :=
-  let fix aux depth t :=
-    match t with 
-    | tVar x' => if x == x' then tRel depth else tVar x'
-    | _ => map_term_with_binders 0 (fun _ => S) aux t
-    end
-  in 
-  aux 0 t.
-
-(** Get the evar id in a term of the form [tEvar _ _]. *)
-Definition get_evar_id (t : term) : evar :=
-  match t with 
-  | tEvar ev _ => ev 
-  | _ => 0
   end.
 
 (** [intro x] works on the main goal : it unifies the goal with a product type 
@@ -220,7 +238,7 @@ Definition intro_tac (basename : ident) : TacticM ident :=
   (* Unify [forall x : ?a, ?b <=? typeof(goal)]. *)
   mlet concl <- main_concl ;;
   mlet unified <- unify_tac UnifFlags.default Cumul (tProd binder a $ abstract name b) concl ;;
-  (if unified then ret tt else fail_tac) ;;
+  (if unified then ret tt else fail_tac $ str "intro_tac : goal is not a product") ;;
   (* Set [?goal := fun x : ?a, ?body] *)
   mlet body <- with_named_context body_nctx (fresh_evar "goal" (Some b)) ;;
   assign_tac goal (tLambda binder a $ abstract name body) ;;
@@ -235,13 +253,11 @@ Definition apply_tac (t : term) : TacticM unit :=
      [t_ty] is the type of [t] applied to the arguments. *)
   let fix loop (args : list term) (t_ty : term) {struct t_ty} : TacticM (list term) :=
     (* Check if we can apply [t] with the evars created so far. *)
-    mlet concl <- main_concl ;;
-    mlet can_apply <- unify_tac UnifFlags.default Cumul t_ty concl ;;
+    mlet can_apply <- unify_tac UnifFlags.default Cumul t_ty =<< main_concl ;;
     if can_apply then ret $ rev args else 
     (* Otherwise, create an evar for the next argument of [t] and recurse. *)
-    (* TODO : weak-head reduce [t_ty]. *)
-    mlet evm <- get_evar_map ;;
-    match whd_evars evm t_ty with 
+    mlet t_ty <- whnf_tac RedFlags.all t_ty ;;
+    match t_ty with 
     | tProd x x_ty t_ty =>
       let ev_name := 
         match x.(binder_name) with 
@@ -252,7 +268,7 @@ Definition apply_tac (t : term) : TacticM unit :=
       mlet ev <- fresh_evar ev_name (Some $ subst0 args x_ty) ;;
       loop (ev :: args) (subst0 [ev] t_ty)
     (* No more arguments : the application has failed. *)
-    | _ => fail_tac 
+    | _ => fail_tac $ str "apply_tac : application failed"
     end 
   in 
   simple_tactic $ fun goal => 
@@ -263,5 +279,82 @@ Definition apply_tac (t : term) : TacticM unit :=
   assign_tac goal (mkApps t args) ;;
   ret (tt, map get_evar_id args).
 
+(** [dest_ind_tac t] checks that [t] is a (declared) inductive applied to _all_ of its 
+    parameters and indices, and returns the various components of [t] :
+    [(mbody, ibody, ind, uinst, params, indices)]. *)
+Definition dest_ind_tac (t : term) : 
+  TacticM (mutual_inductive_body * one_inductive_body * inductive * 
+           Instance.t * list term * list term) :=
+  (* Don't forget to weak head normalize [t]. *)
+  mlet t <- whnf_tac RedFlags.all t ;;
+  match t with 
+  | tApp (tInd ind uinst) args =>
+    (* Lookup the inductive. *)
+    mlet env <- get_global_env ;;
+    match lookup_inductive env ind with 
+    | Some (mbody, ibody) => 
+      (* Extract the parameters and indices. *)
+      if context_assumptions mbody.(ind_params) + context_assumptions ibody.(ind_indices) <=? #|args| 
+      then 
+        let (params, indices) := chop mbody.(ind_npars) args in
+        ret (mbody, ibody, ind, uinst, params, indices)
+      else fail_tac $ str "dest_ind_tac : inductive is not fully applied"
+    | None => fail_tac $ str "dest_ind_tac : inductive is not declared"
+    end
+  | _ => fail_tac $ str "dest_ind_tac : not an inductive"
+  end.
+  
 (** [constructor_tac n] works on the main goal : if it is an inductive,
     it applies the [n]-th constructor of this inductive. *)
+Definition constructor_tac (n : nat) : TacticM unit :=
+  with_main_context $
+  (* Check the goal is an inductive fully applied to its parameters and indices. *)
+  mlet (mbody, ibody, ind, uinst, _, _) <- dest_ind_tac =<< main_concl ;;
+  (* Check the constructor index is valid. *)
+  (if n <? #|ibody.(ind_ctors)| then ret tt 
+  else fail_tac $ str "constructor_tac : invalid constructor index") ;;
+  (* Apply the constructor, with the same universe instance as the goal. *)
+  apply_tac (tConstruct ind n uinst).
+
+(** [destruct_tac t] works on the main goal : if [t] is of inductive type,
+    it inserts a case expression on [t]. It creates a subgoal for each
+    branch. It does not handle dependent elimination (yet). *)
+Definition destruct_tac (t : term) : TacticM unit :=
+  mlet concl <- main_concl ;;
+  simple_tactic $ fun goal =>
+  (* Check the type of [t] is an inductive applied to its parameters and indices. *)
+  mlet (mbody, ibody, ind, uinst, params, indices) <- dest_ind_tac =<< typeof_tac t ;;
+  (* Create a subgoal for each branch. *)
+  mlet subgoals <- 
+    monad_map 
+      (fun ctor => 
+        (* The subgoal is a product, i.e. we don't prematurely introduce variables. *)
+        let ctx := smash_context [] ctor.(cstr_args) in
+        fresh_evar "u" $ Some $ it_mkLambda_or_LetIn ctx concl)
+      ibody.(ind_ctors)
+  ;;
+  (* Assign a case expression to the current goal. *)
+  let ci := 
+    {| ci_ind := ind 
+    ;  ci_npar := mbody.(ind_npars)
+    ;  ci_relevance := ibody.(ind_relevance) |}
+  in
+  (* The return type of the match is simply the conclusion of the main goal. *)
+  let pred := 
+    {| puinst := uinst 
+    ;  pparams := params 
+    ;  pcontext := map decl_name ibody.(ind_indices)
+    ;  preturn := concl |}
+  in
+  let branches :=
+    map2 
+      (fun sg ctor => 
+        (* Don't forget to apply each branch evar to the arguments of the constructor. *)
+        {| bcontext := map decl_name ctor.(cstr_args) 
+        ;  bbody := mkApps sg $ rev $ mapi (fun i _ => tRel i) ctor.(cstr_args) |}) 
+      subgoals 
+      ibody.(ind_ctors)
+  in
+  assign_tac goal (tCase ci pred t branches) ;;
+  (* Return the list of new goals. *)
+  ret (tt, map get_evar_id subgoals).
